Mergeable interfaces
Considering the mergeability of states and performing actual merges are
operations which are conceived to be meaningfully applied in very
specific conditions. To begin to express these conditions, the link with
program interfaces is established.

The new condition is added to the mergeable_states relation, new
hypotheses introduced as needed and changes propagated. Modulo the
temporary omissions in (partial) proofs introduced in the previous
commit, only the (painful) attention required by automatically named
hypotheses need to be revisited in addition to the obvious changes. No
problems are observed in the approach so far.

Intermediate/PS.v
@@ -349,8 +349,23 @@ Inductive mergeable_stacks : stack -> stack -> Prop :=
 Definition mergeable_memories (mem1 mem2: Memory.t): Prop :=
   fdisjoint (domm mem1) (domm mem2).
 
+Definition mergeable_interfaces (ctx1 ctx2: Program.interface) : Prop :=
+  linkable ctx1 ctx2 /\
+  closed_interface (unionm ctx1 ctx2).
+
+Lemma mergeable_interfaces_sym ctx1 ctx2 :
+  mergeable_interfaces ctx1 ctx2 ->
+  mergeable_interfaces ctx2 ctx1.
+Proof.
+  intros [Hlinkable Hclosed].
+  split.
+  - apply (linkable_sym Hlinkable).
+  - apply (closed_interface_sym _ _ Hclosed).
+Qed.
+
 Inductive mergeable_states (ctx1 ctx2: Program.interface): state -> state -> Prop :=
 | mergeable_states_first: forall ips1 ips2,
+    mergeable_interfaces ctx1 ctx2 ->
     is_program_component ips1 ctx1 ->
     is_context_component ips2 ctx2 ->
     state_component ips1 = state_component ips2 ->
@@ -358,6 +373,7 @@ Inductive mergeable_states (ctx1 ctx2: Program.interface): state -> state -> Pro
     mergeable_memories (state_memory ips1) (state_memory ips2) ->
     mergeable_states ctx1 ctx2 ips1 ips2
 | mergeable_states_second: forall ips1 ips2,
+    mergeable_interfaces ctx1 ctx2 ->
     is_context_component ips1 ctx1 ->
     is_program_component ips2 ctx2 ->
     state_component ips1 = state_component ips2 ->
@@ -405,10 +421,15 @@ Lemma mergeable_states_sym:
     PS.mergeable_states (prog_interface p) (prog_interface c) s2 s1.
 Proof.
   intros p c s1 s2 Hp_wf Hc_wf Hlink Hmergeable.
-  inversion Hmergeable; subst;
-  do 2 (constructor; auto;
-        [ apply mergeable_stacks_sym; auto
-        | apply mergeable_memories_sym; auto ]).
+  inversion Hmergeable; subst.
+  - apply mergeable_states_second; auto.
+    + apply mergeable_interfaces_sym; assumption.
+    + apply mergeable_stacks_sym; assumption.
+    + apply mergeable_memories_sym; assumption.
+  - apply mergeable_states_first; auto.
+    + apply mergeable_interfaces_sym; assumption.
+    + apply mergeable_stacks_sym; assumption.
+    + apply mergeable_memories_sym; assumption.
 Qed.
 
 Definition merge_stack_frames (frames: PartialPointer.t * PartialPointer.t): PartialPointer.t :=
